@prefix elmo: <http://dotwebstack.org/def/elmo#>.
@prefix elmo-sp: <http://dotwebstack.org/def/elmo/storage-protocol/>.
@prefix xsd: <http://www.w3.org/2001/XMLSchema#>.
@prefix rdf: <http://www.w3.org/1999/02/22-rdf-syntax-ns#>.
@prefix rdfs: <http://www.w3.org/2000/01/rdf-schema#>.
@prefix owl: <http://www.w3.org/2002/07/owl#>.
@prefix sh: <http://www.w3.org/ns/shacl#>.
@prefix void: <http://rdfs.org/ns/void#>.
@prefix sh: <http://www.w3.org/ns/shacl#>.
@prefix xhtml: <http://www.w3.org/1999/xhtml/vocab#>.
@prefix xs: <http://www.w3.org/2001/XMLSchema#>.
@prefix elmoshape: <http://bp4mc2.org/elmo/def/>.
@prefix yed: <http://bp4mc2.org/yed/def#>.
@prefix rdf: <http://www.w3.org/1999/02/22-rdf-syntax-ns#>.
@prefix rdfs: <http://www.w3.org/2000/01/rdf-schema#>.
@prefix skos: <http://www.w3.org/2004/02/skos/core#>.
@prefix elmo: <http://dotwebstack.org/def/elmo#>.
@prefix elmo-schemes: <http://dotwebstack.org/def/elmo/>.
@prefix elmo-rt: <http://dotwebstack.org/def/elmo/result-type/>.

GRAPH elmo:Config {
  elmo:SparqlBackend rdfs:subClassOf elmo:Backend .
}

GRAPH elmo:Config {
  # =========
  # Resulttypes
  #
  elmo-schemes:result-types a skos:ConceptScheme;
    rdfs:label "Result types"@en;
  .

  elmo-rt:Tuple a elmo:ResultType;
    skos:inScheme elmo-schemes:result-types;
    rdfs:label "Tuple";
    rdfs:comment "The result contains tuples (an ordered list of bindingsets), for example the result of a SELECT query."
  .
  elmo-rt:Graph a elmo:ResultType;
    skos:inScheme elmo-schemes:result-types;
    rdfs:label "Graph";
    rdfs:comment "The result is a graph (a set of triples), for example the result of a CONSTRUCT query."
  .
}


GRAPH elmo:Config {
# ======
#
# Vocabulary and dataset
#
# ======
<http://bp4mc2.org/elmo/def#> a	owl:Ontology;
	rdfs:label "The ELMO vocabulary";
	rdfs:comment "The vocabulary to configure the Linked Data Theatre. ELMO stands for Extendible Lightweight Model Ontology.";
.
<http://bp4mc2.org/elmo/def> a	void:Dataset;
	rdfs:label "The dataset containing the ELMO vocabulary";
.

# ======
#
# PART
#
# ======
elmo:Part a owl:Class;
	rdfs:label "Part"@en;
	rdfs:label "Onderdeel"@nl;
	rdfs:comment "The class of UI parts, as a part of a Representation";
	rdfs:comment "De klasse van UI onderdelen, als onderdeel van een Representatie";
.
elmoshape:Part a sh:NodeShape;
	sh:targetClass elmo:Part;
	sh:name "elmo:Part";
	sh:property [
		sh:path elmo:fragment;
		sh:name "elmo:fragment";
		sh:nodeKind sh:IRI;
		sh:class elmo:RepresentationFragment;
	];
	sh:property [
		sh:path elmo:query;
		sh:name "elmo:query";
		sh:nodeKind sh:Literal;
		sh:maxCount 1;
	];
	sh:property [
		sh:path elmo:query;
		sh:name "elmo:query";
		sh:nodeKind sh:IRI;
		sh:class elmo:Query;
		sh:maxCount 1;
	];
	sh:property [
		sh:path elmo:index;
		sh:name "elmo:index";
		sh:nodeKind sh:Literal;
		sh:maxCount 1;
	];
	sh:property [
		sh:path elmo:data;
		sh:name "elmo:data";
		sh:nodeKind sh:BlankNode;
		sh:maxCount 1;
	];
	sh:property [
		sh:path elmo:endpoint;
		sh:name "elmo:endpoint";
		sh:nodeKind sh:IRI;
		sh:maxCount 1;
	];
	sh:property [
		sh:path elmo:layer;
		sh:name "elmo:layer";
		sh:nodeKind sh:IRI;
		sh:class elmo:Layer;
		sh:maxCount 1;
	];
	sh:property [
		sh:path elmo:appearance;
		sh:name "elmo:appearance";
		sh:nodeKind sh:IRI;
		sh:class elmo:Appearance;
		sh:maxCount 1;
	];
	sh:property [
		sh:path xhtml:stylesheet;
		sh:name "xhtml:stylesheet";
		sh:nodeKind sh:Literal;
		sh:maxCount 1;
	];
.

# ======
#
# REPRESENTATION
#
# ======
elmo:Representation a owl:Class;
	rdfs:subClassOf elmo:Part;
	rdfs:label "Representation"@en;
	rdfs:label "Representatie"@nl;
	rdfs:comment "The class of representations of a resource"@en;
	rdfs:comment "De klasse van representaties van een resource"@nl;
.
elmoshape:Representation a sh:NodeShape;
	sh:targetClass elmo:Representation;
	sh:name "elmo:Representation";
	sh:property [
		sh:path elmo:url-pattern;
		sh:name "elmo:url-pattern";
		sh:nodeKind sh:Literal;
	];
	sh:property [
		sh:path elmo:uri-pattern;
		sh:name "elmo:uri-pattern";
		sh:nodeKind sh:Literal;
	];
	sh:property [
		sh:path elmo:applies-to;
		sh:name "elmo:applies-to";
		sh:nodeKind sh:BlankNode;
	];
	sh:property [
		sh:path elmo:contains;
		sh:name "elmo:contains";
		sh:nodeKind sh:IRI;
		sh:class elmo:Part;
	];
	sh:property [
		sh:path elmo:queryForm;
		sh:name "elmo:queryForm";
		sh:nodeKind sh:IRI;
		sh:maxCount 1;
		sh:class elmo:Form;
	];
.

# ======
#
# FRAGMENT
#
# ======
elmo:Fragment a owl:Class;
	rdfs:label   "Fragment"@en;
	rdfs:label   "Fragment"@nl;
	rdfs:comment "The class of fragments"@en;
	rdfs:comment "De klasse van fragmenten"@nl;
.
elmo:RepresentationFragment a owl:Class;
	rdfs:subClassOf elmo:Fragment;
	rdfs:label   "Fragment"@en;
	rdfs:label   "Fragment"@nl;
	rdfs:comment "The class of fragments of a representation"@en;
	rdfs:comment "De klasse van fragmenten van een representatie"@nl;
.
elmo:FormFragment a owl:Class;
	rdfs:subClassOf elmo:Fragment;
	rdfs:label   "Fragment"@en;
	rdfs:label   "Fragment"@nl;
	rdfs:comment "The class of fragments of a form"@en;
	rdfs:comment "De klasse van fragmenten van een formulier"@nl;
.
elmo:YedFragment a owl:Class;
	rdfs:subClassOf elmo:RepresentationFragment;
	rdfs:label   "Fragment"@en;
	rdfs:label   "Fragment"@nl;
	rdfs:comment "The class of fragments of a yED representation"@en;
	rdfs:comment "De klasse van fragmenten van een yED representatie"@nl;
.
elmoshape:Fragment a sh:NodeShape;
	sh:targetClass elmo:Fragment;
	sh:name "elmo:Fragment";
	sh:property [
		sh:path rdfs:label;
		sh:name "rdfs:label";
		sh:nodeKind sh:Literal;
		sh:datatype xs:string;
	];
	sh:property [
		sh:path elmo:applies-to;
		sh:name "elmo:applies-to";
		sh:nodeKind sh:Literal;
	];
	sh:property [
		sh:path elmo:index;
		sh:name "elmo:index";
		sh:nodeKind sh:Literal;
	];
.
elmoshape:RepresentationFragment a sh:NodeShape;
	sh:targetClass elmo:RepresentationFragment;
	sh:name "elmo:RepresentationFragment";
	sh:property [
		sh:path elmo:appearance;
		sh:name "elmo:appearance";
		sh:nodeKind sh:IRI;
		sh:class elmo:Appearance;
	];
	sh:property [
		sh:path elmo:glossary;
		sh:name "elmo:glossary";
		sh:nodeKind sh:IRI;
		sh:class elmo:Part;
	];
	sh:property [
		sh:path xhtml:stylesheet;
		sh:name "xhtml:stylesheet";
		sh:nodeKind sh:Literal;
	];
	sh:property [
		sh:path xhtml:link;
		sh:name "xhtml:link";
		sh:nodeKind sh:IRI;
	];
	sh:property [
		sh:path rdf:value;
		sh:name "rdf:value";
	];
.
elmoshape:FormFragment a sh:NodeShape;
	sh:targetClass elmo:FormFragment;
	sh:name "elmo:FormFragment";
	sh:property [
		sh:path elmo:constraint;
		sh:name "elmo:constraint";
		sh:nodeKind sh:IRI;
		sh:class elmo:Constraint;
	];
	sh:property [
		sh:path elmo:valueDatatype;
		sh:name "elmo:valueDatatype";
	];
	sh:property [
		sh:path elmo:valueFormat;
		sh:name "elmo:valueFormat";
	];
	sh:property [
		sh:path elmo:valuesFrom;
		sh:name "elmo:valuesFrom";
	];
.
elmoshape:YedFragment a sh:NodeShape;
	sh:targetClass elmo:YedFragment;
	sh:name "elmo:YedFragment";
	sh:property [
		sh:path yed:backgroundColor;
		sh:name "yed:backgroundColor";
		sh:nodeKind sh:Literal;
	];
	sh:property [
		sh:path yed:edge;
		sh:name "yed:edge";
		sh:nodeKind sh:Literal;
	];
	sh:property [
		sh:path yed:line;
		sh:name "yed:line";
		sh:nodeKind sh:Literal;
	];
	sh:property [
		sh:path yed:sourceArrow;
		sh:name "yed:sourceArrow";
		sh:nodeKind sh:Literal;
	];
	sh:property [
		sh:path yed:targetArrow;
		sh:name "yed:targetArrow";
		sh:nodeKind sh:Literal;
	];
.

# ======
#
# CONTAINER
#
# ======
elmo:Container a owl:Class;
	rdfs:label   "Container"@en;
	rdfs:label   "Container"@nl;
	rdfs:comment "The regular container. Updates to this container will be inserted into the graph with the same URI as the container";
	rdfs:comment "De normale container. Toevoegingen aan deze container worden toegevoegd aan de graaf met dezelfde URI als de container";
.
elmoshape:Container a sh:NodeShape;
	sh:targetClass elmo:Container;
	sh:name "elmo:Container";
	sh:property [
		sh:path rdfs:label;
		sh:name "rdfs:label";
		sh:nodeKind sh:IRI;
		sh:class elmo:Translator;
	];
	sh:property [
		sh:path elmo:representation;
		sh:name "elmo:representation";
		sh:nodeKind sh:IRI;
	];
	sh:property [
		sh:path elmo:contains;
		sh:name "elmo:contains";
		sh:nodeKind sh:IRI;
		sh:class elmo:Part;
	];
	sh:property [
		sh:path elmo:translator;
		sh:name "elmo:translator";
		sh:nodeKind sh:IRI;
		sh:class elmo:Translator;
	];
	sh:property [
		sh:path elmo:replaces;
		sh:name "elmo:replaces";
		sh:nodeKind sh:IRI;
	];
	sh:property [
		sh:path elmo:updates;
		sh:name "elmo:updates";
		sh:nodeKind sh:IRI;
	];
	sh:property [
		sh:path elmo:partOf;
		sh:name "elmo:partOf";
		sh:nodeKind sh:IRI;
	];
	sh:property [
		sh:path elmo:query;
		sh:name "elmo:query";
		sh:nodeKind sh:Literal;
	];
	sh:property [
		sh:path elmo:query;
		sh:name "elmo:query";
		sh:nodeKind sh:IRI;
		sh:class elmo:Query;
	];
.

# ======
#
# QUERY
#
# ======
elmo:Query a owl:Class;
	rdfs:label   "Query"@en;
	rdfs:label   "Query"@nl;
	rdfs:comment "defines the SPARQL query that corresponds with the particular representation"@en;
	rdfs:comment "definieert de SPARQL query die overeen komt met de betreffende representatie"@nl;
.
elmoshape:Query a sh:NodeShape;
	sh:targetClass elmo:Query;
	sh:name "elmo:Query";
	sh:property [
		sh:path elmo:query;
		sh:name "elmo:query";
		sh:nodeKind sh:Literal;
		sh:maxCount 1;
	];
.

# ======
#
# FORM
#
# ======
elmo:Form			a	owl:Class;
	rdfs:label			"Form"@en;
	rdfs:label			"Formulier"@nl;
	rdfs:comment		"The class of UI forms, from which a user can enter some URL parameters"@en;
	rdfs:comment		"De klasse van UI formulieren, van waaruit een gebruiker bepaalde URL parameters kan invoeren"@nl;
.
elmoshape:Form a sh:NodeShape;
	sh:targetClass elmo:Form;
	sh:name "elmo:Form";
	sh:property [
		sh:path elmo:fragment;
		sh:class elmo:FormFragment;
		sh:name "elmo:fragment";
		sh:nodeKind sh:Iri;
	];
.

# ======
#
# LAYER
#
# ======
elmo:Layer			a	owl:Class;
	rdfs:label			"Layer"@en;
	rdfs:label			"Laag"@nl;
	rdfs:comment		"The class of layers. A representation is located at a specific layer"@en;
	rdfs:comment		"De klasse van lagen. Een verschijning bevindt zich op een specifieke laag"@nl;
.
elmoshape:Layer a sh:NodeShape;
	sh:targetClass elmo:Layer;
	sh:name "elmo:Layer";
.

# ======
#
# APPEARANCE
#
# ======
elmo:Appearance		a	owl:Class;
	rdfs:label			"Appearance"@en;
	rdfs:label			"Verschijning"@nl;
	rdfs:comment		"The generic appearance class. Implementations should use a subclass of this appearance."@en;
	rdfs:comment		"De generieke verschijningsklasse. Implementaties behoren een subklasse van deze verschijning te gebruiken."@nl;
.
elmoshape:Appearance a sh:NodeShape;
	sh:targetClass elmo:Appearance;
	sh:name "elmo:Appearance";
.

### Classes ###
elmo:VersionContainer	a	owl:Class;
	rdfs:label			"Versioned container"@en;
	rdfs:label			"Geversioneerde container"@nl;
	rdfs:subClassOf		elmo:Container;
	rdfs:comment		"The versioned container. Update to this container will be inserted into a versioned graph and to regular graph";
	rdfs:comment		"De geversioneerde container. Toevoegingen aan deze container worden toegevoegd aan een geversioneerde graaf en naar de normale graaf";
.
elmo:Translator		a	owl:Class;
	rdfs:label			"Translator"@en;
	rdfs:label			"Translator"@nl;
	rdfs:comment		"The generic translator class. Implementations should use a subclass of this translator."@en;
	rdfs:comment		"The generieke vertalerklasse. Implementaties behoren een subklasse van deze vertaler te gebruiken."@nl;
.
elmo:Constraint		a	owl:Class;
	rdfs:label			"Constraint"@en;
	rdfs:label			"Beperking"@nl;
	rdfs:comment		"The class of constraints. A constraint can be set on a fragment of a form"@en;
	rdfs:comment		"The klasse van beperkingen. Een beperking kan gezet worden op een fragment van een formulier"@nl;
.
elmo:GeoLocator		a	rdfs:Class;
	rdfs:label			"Geo locator"@en;
	rdfs:label			"Geo aanwijzer"@nl;
	rdfs:comment		"A resource that is a GeoLocator will be used to center a geographical map to the coordinates of the GeoLocator"@en;
	rdfs:comment		"Een resource die een GeoLocator is, wordt gebruikt om de geografische map te centreren op de coordinaten van de GeoLocator"@nl;
.
elmo:Production		a	owl:Class;
	rdfs:label			"Production"@en;
	rdfs:label			"Productie"@nl;
	rdfs:comment		"The class of productions. A production is a list of scenes that creates or deletes a set of triples"@en;
	rdfs:comment		"The klasse van producties. Een productie is een lijst van scenes die een verzameling triples toevoegen of verwijderen"@nl;
.
elmo:Scene			a	owl:Class;
	rdfs:label			"Scene"@en;
	rdfs:label			"Scene"@nl;
	rdfs:comment		"The class of scenes. A scene is a single transformation of the triplestore. A scene defines a single SPARUL statement"@en;
	rdfs:comment		"De klasse van scenes. Een scene is een enkelvoudige transformatie van de triplestore. Een scene definieert een enkelvoudig SPARUL statement"@nl;
.

# Appearance subclasses #
elmo:CoreAppearance		a	owl:Class;
	rdfs:subClassOf			elmo:Appearance;
	rdfs:label				"Core appearance"@en;
	rdfs:label				"Kernverschijning"@nl;
	rdfs:comment			"A core appearance. Six appearances are part of the core of the LDT."@en;
	rdfs:comment			"Een kernverschijning. Zes verschijningen zijn onderdeel van de kern van het LDT"@nl;
.
elmo:ExtensionAppearance	a	owl:Class;
	rdfs:subClassOf			elmo:Appearance;
	rdfs:label				"Extension appearance"@en;
	rdfs:label				"Aanvullende verschijning"@nl;
	rdfs:comment			"An extension appearance. The LDT can be extended with a particular appearance, which should always be a subclass of the extension appearance"@en;
	rdfs:comment			"Een aanvullende verschijning. Het LDT kan aangevuld worden met een specifieke verschijning, die altijd een subklasse behoord te zijn van de aanvullende verschijning"@nl;
.
elmo:FragmentAppearance	a	owl:Class;
	rdfs:subClassOf			elmo:Appearance;
	rdfs:label				"Fragment appearance"@en;
	rdfs:label				"Fragmentverschijning"@nl;
	rdfs:comment			"An appearance used for fragments."@en;
	rdfs:comment			"Een verschijning die voor fragmenten wordt gebruikt"@nl;
.
elmo:TableAppearance	a	owl:Class;
	rdfs:subClassOf			elmo:CoreAppearance;
	rdfs:label				"Table appearance"@en;
	rdfs:label				"Tabelverschijning"@nl;
.
elmo:ShortTableAppearance	a	owl:Class;
	rdfs:subClassOf			elmo:TableAppearance;
	rdfs:label				"Short table appearance"@en;
	rdfs:label				"Minimale tabelverschijning"@nl;
.
elmo:ContentAppearance	a	owl:Class;
	rdfs:subClassOf			elmo:CoreAppearance;
	rdfs:label				"Content appearance"@en;
	rdfs:label				"Eigenschappenverschijning"@nl;
.
elmo:HeaderAppearance	a	owl:Class;
	rdfs:subClassOf			elmo:CoreAppearance;
	rdfs:label				"Header appearance"@en;
	rdfs:label				"Kopverschijning"@nl;
	rdfs:comment			"An appearance used for the header of a page. Usually contains an image and a pay-off text."@en;
	rdfs:comment			"Een verschijning te gebruiken voor de kop van een pagina. Meestal bevat deze een plaatje en een pay-off tekst."@nl;
.
elmo:NavbarAppearance	a	owl:Class;
	rdfs:subClassOf			elmo:CoreAppearance;
	rdfs:label				"Navigation bar appearance"@en;
	rdfs:label				"Navigatiebalkverschijning"@nl;
	rdfs:comment			"An appearance used for the navigation bar"@en;
	rdfs:comment			"Een verschijning te gebruiken voor een navigatiebalk."@nl;
.
elmo:NavbarSearchAppearance	a	owl:Class;
	rdfs:subClassOf			elmo:NavbarAppearance;
	rdfs:label				"Navigation bar with search appearance"@en;
	rdfs:label				"Navigatiebalkverschijning met zoeken"@nl;
	rdfs:comment			"An appearance used for the navigation bar, including a search form"@en;
	rdfs:comment			"Een verschijning te gebruiken voor een navigatiebalk, inclusief een zoekformulier."@nl;
.
elmo:HiddenAppearance	a	owl:Class;
	rdfs:subClassOf			elmo:CoreAppearance;
	rdfs:label				"Hidden appearance"@en;
	rdfs:label				"Verborgen verschijning"@nl;
	rdfs:comment			"An appearance that is actually hidden. These seems paradoxical, but can be usefull if some data should not be shown in a html view, but should be used otherwise"@en;
	rdfs:comment			"Een verschijning die verborgen is. Dit lijkt paradoxaal, maar kan bruikbaar zijn indien bepaalde gegevens niet getoond moeten worden in de html weergave, maar op een andere manier worden gebruikt"@nl;
.
elmo:LoginAppearance	a	owl:Class;
	rdfs:subClassOf			elmo:ExtensionAppearance;
	rdfs:label				"Login appearance"@en;
	rdfs:label				"Login verschijning"@nl;
	rdfs:comment			"An appearance used for a login page"@en;
	rdfs:comment			"Een verschijning te gebruiken voor een login pagina"@nl;
.
elmo:CarouselAppearance	a	owl:Class;
	rdfs:subClassOf			elmo:ContentAppearance;
	rdfs:label				"Carousel appearance"@en;
	rdfs:label				"Carrouselverschijning"@nl;
.
elmo:IndexAppearance	a	owl:Class;
	rdfs:subClassOf			elmo:CoreAppearance;
	rdfs:label				"Index appearance"@en;
	rdfs:label				"Indexverschijning"@nl;
.
elmo:HtmlAppearance		a	owl:Class;
	rdfs:subClassOf			elmo:ExtensionAppearance;
	rdfs:label				"HTML appearance"@en;
	rdfs:label				"HTML verschijning"@nl;
	rdfs:comment			"An appearance used for displaying a piece of html. Mostly used for literal representations of a piece of text"@en;
	rdfs:comment			"Een verschijning te gebruiken voor het tonen van een stukje html. Meestal gebruikt voor letterlijke representaties van een stukje tekst"@nl;
.
elmo:GraphAppearance	a	owl:Class;
	rdfs:subClassOf			elmo:ExtensionAppearance;
	rdfs:label				"Graph appearance"@en;
	rdfs:label				"Grafische verschijning"@nl;
.
elmo:TextAppearance	a	owl:Class;
	rdfs:subClassOf			elmo:ExtensionAppearance;
	rdfs:label				"Text appearance"@en;
	rdfs:label				"Tekstuele verschijning"@nl;
.
elmo:FormAppearance	a	owl:Class;
	rdfs:subClassOf			elmo:ExtensionAppearance;
	rdfs:label				"Form appearance"@en;
	rdfs:label				"Formulierverschijning"@nl;
.
elmo:GeoAppearance	a	owl:Class;
	rdfs:subClassOf			elmo:ExtensionAppearance;
	rdfs:label				"Geographical appearance"@en;
	rdfs:label				"Geografische verschijning"@nl;
.
elmo:ImageAppearance	a	owl:Class;
	rdfs:subClassOf			elmo:GraphAppearance;
	rdfs:label				"Image appearance"@en;
	rdfs:label				"Plaatjes-verschijning"@nl;
.
elmo:ChartAppearance	a	owl:Class;
	rdfs:subClassOf			elmo:ExtensionAppearance;
	rdfs:label				"Chart appearance"@en;
	rdfs:label				"Diagramverschijning"@nl;
.
elmo:TextSearchAppearance	a	owl:Class;
	rdfs:subClassOf			elmo:TableAppearance;
	rdfs:label				"Text search appearance"@en;
	rdfs:label				"Zoeken naar tekst verschijning"@nl;
.
elmo:GlobalLink			a	owl:Class;
	rdfs:subClassOf			elmo:FragmentAppearance;
	rdfs:label				"Global link"@en;
	rdfs:label				"Internetverwijzing"@nl;
	rdfs:comment			"A global links states that a fragment should contain hyperlinks to the real URL, even if its outside the Linked Data Theatre application"@en;
	rdfs:comment			"Een internetverwijzing stelt dat een fragment hyperlinks bevat die verwijzen naar de echte URL, zelfs als deze URL zich bevindt buiten de Linked Data Theater applicatie"@nl;
.
elmo:FilteredGlossaryAppearance	a	owl:Class;
	rdfs:subClassOf			elmo:FragmentAppearance;
	rdfs:label				"Filtered glossary appearance";
	rdfs:label				"Gefilterde woordenlijst verschijning";
.
elmo:SubmitAppearance	a	owl:Class;
	rdfs:subClassOf			elmo:FragmentAppearance;
	rdfs:label				"Submit appearance"@en;
	rdfs:label				"Submit verschijning"@nl;
	rdfs:comment			"A fragment that appears as a submit button"@en;
	rdfs:comment			"Een fragment dat er uit ziet als een submit-knop"@nl;
.
elmo:CesiumAppearance	a	owl:Class;
	rdfs:subClassOf			elmo:ExtensionAppearance;
	rdfs:label				"Cesium appearance"@en;
	rdfs:label				"Cesium-verschijning"@nl;
	rdfs:comment			"An appearance using the Cesium framework"@en;
	rdfs:comment			"Een verschijning die het Cesium raamwerk gebruikt"@nl;
.
elmo:VocabularyAppearance a owl:Class;
	rdfs:subClassOf			elmo:ExtensionAppearance;
	rdfs:label				"Vocabulary appearance"@en;
	rdfs:label				"Vocabulaire-verschijning"@nl;
	rdfs:comment			"An appearance designed for representing a vocabulary or ontology"@en;
	rdfs:comment			"Een verschijning die specifiek is ontworpen om een vocabulaire of ontologie te vertonen"@nl;
.

elmo:Style				a	owl:Class;
	rdfs:label				"Style"@en;
	rdfs:label				"Stijl"@nl;
	rdfs:comment			"The class of CSS styles (to format a fragment or a representation)."@en;
	rdfs:comment			"De klasse van CSS stijlen (om een fragment of een represntatie te formatteren)."@nl;
.

# Layers #
elmo:TopLayer		a	elmo:Layer;
	rdfs:label			"top layer"@en;
	rdfs:label			"bovenste laag"@nl;
	rdfs:comment		"The top layer. Representations located at this layer are always used"@en;
	rdfs:comment		"De bovenste laag. Representaties die op deze laag bevinden worden altijd gebruikt"@nl;
.
elmo:DefaultLayer	a	elmo:Layer;
	rdfs:label			"default layer"@en;
	rdfs:label			"standaardlaag"@nl;
	rdfs:comment		"The default layer. The default layer is located in the middle between the top and the bottom layer. Representations without an explicitly defined layer are located at the default layer"@en;
	rdfs:comment		"De standaardlaag. De standaardlaag bevindt zich in het midden tussen de bovenste en onderste laag. Representaties zonder een expliciet gedefinieerde laag bevinden zich op de standaardlaag"@nl;
.
elmo:BottomLayer	a	elmo:Layer;
	rdfs:label			"bottom layer"@en;
	rdfs:label			"onderste laag"@nl;
	rdfs:comment		"The bottom layer. Representations located at this layer are only used if no other layer is available"@en;
	rdfs:comment		"De onderste laag. Representaties die op deze laag bevinden worden alleen gebruikt als er geen andere laag beschikbaar is"@nl;
.

# Translators #
elmo:SimpleTranslator	a	owl:Class;
	rdfs:subClassOf		elmo:Translator;
	rdfs:label			"Simple translator";
	rdfs:label			"Eenvoudige vertaler";
	rdfs:comment		"Translates XML to a simple RDF format. Most usable for debugging purposes"@en;
	rdfs:comment		"Vertaalt XML in een simpel RDF formaat. Bruikbaar voor debugging"@nl;
.
elmo:XMI21Translator	a	owl:Class;
	rdfs:subClassOf		elmo:Translator;
	rdfs:label			"XMI2.1 translator";
	rdfs:label			"XMI2.1 vertaler";
	rdfs:comment		"Translates XMI2.1 to corresponding linked data (uml schema)"@en;
	rdfs:comment		"Vertaalt XMI2.1 naar overeenkomstige linked data (uml schema)"@nl;
.
elmo:SimpleExcelTranslator	a owl:Class;
	rdfs:subClassOf		elmo:Translator;
	rdfs:label			"Simple excel translator";
	rdfs:label			"Eenvoudige excel vertaler";
	rdfs:comment		"Simple translator for excel files. Assumes only one excel worksheet and a header row containing the properties."@en;
	rdfs:comment		"Eenvoudige vertaler voor excel bestanden. Veronderstelt slechts 1 excel werkblad en een kopregel waarin de properties staan."@nl;
.
elmo:GenericExcelTranslator	a owl:Class;
	rdfs:subClassOf		elmo:Translator;
	rdfs:label			"Generic excel translator";
	rdfs:label			"Generieke excel vertaler";
	rdfs:comment		"Generic translator for excel files. Translates an excel file to a SPARQL result set"@en;
	rdfs:comment		"Generieke vertaler voor excel bestanden. Vertaalt een excel bestand naar een SPARQL result set"@nl;
.

# Constraints #
elmo:MandatoryConstraint	a	elmo:Constraint;
	rdfs:label			"Mandatory constraint"@en;
	rdfs:label			"Verplichting"@nl;
	rdfs:comment		"States that a fragment of a form is mandatory"@en;
	rdfs:comment		"Stelt dat een fragment van een formulier verplicht is"@nl;
.
elmo:OneOfGroupConstraint	a	elmo:Constraint;
	rdfs:label			"One value from a group constraint"@en;
	rdfs:label			"Een waarde uit een groep beperking"@nl;
	rdfs:comment		"States that a fragment of a form should contain one value from a predefined group of values"@en;
	rdfs:comment		"stelt dat een fragment van een formulier een waarde moet bevatten uit een vooraf gedefinieerde groep van waarden"@nl;
.

# Styles #
elmo:HiddenStyle	a	elmo:Style;
	rdfs:label			"Hidden style"@en;
	rdfs:label			"Verborgen stijl"@nl;
	rdfs:comment		"A style that makes the content hidden."@en;
	rdfs:comment		"Een stijl die de inhoud verborgen maakt."@nl;
.

### Properties ###

elmo:applies-to		a	owl:DatatypeProperty;
	rdfs:label			"applies to"@en;
	rdfs:label			"van toepassing op"@nl;
	rdfs:comment		"states that a (fragment of a) representation applies to a certain resource. The range of applies-to can be the resource itself or a blank-node profile (for example: applies-to/rdf:type owl:Class states that the representation applies to all resource of rdf:type owl:Class)"@en;
	rdfs:comment		"stelt dat een (fragment van een) representatie van toepassing is op een bepaalde resource. Het bereik van van-toepassing-op kan de resource zelf zijn, of een blank-node profiel (bijvoorbeeld: applies-to/rdf:type owl:Class stelt dat de representatie van toepassing is op alle resources van rdf:type owl:Class)"@nl;
.
elmo:url-pattern	a	owl:DatatypeProperty;
	rdfs:label			"url-pattern"@en;
	rdfs:label			"url-patroon"@nl;
	rdfs:comment		"states that a representation applies to all urls with a certain regex pattern"@en;
	rdfs:comment		"stelt dat een representatie van toepassing is op een bepaald regex patroon"@nl;
.
elmo:uri-pattern	a	owl:DatatypeProperty;
	rdfs:label			"uri-pattern"@en;
	rdfs:label			"uri-patroon"@nl;
	rdfs:comment		"states that a representation applies to all resources with a certain regex pattern (for its URI)"@en;
	rdfs:comment		"stelt dat een representatie van toepassing is op alle resources met een bepaald regex patroon (voor de URI van die resource)"@nl;
.
elmo:query			a	owl:DatatypeProperty;
	rdfs:label			"query"@en;
	rdfs:label			"query"@nl;
	rdfs:comment		"defines the SPARQL query that corresponds with the particular representation"@en;
	rdfs:comment		"definieert de SPARQL query die overeen komt met de betreffende representatie"@nl;
.
elmo:data		a	owl:ObjectProperty;
	rdfs:label			"data"@en;
	rdfs:label			"gegevens"@nl;
	rdfs:comment		"defines the data associated with the representation. This data is used instead of the result of the SPARQL query"@en;
	rdfs:comment		"definieert de gegevens die behoren bij de representatie. Deze gegevens worden gebruikt in plaats van het resultaat van de SPARQL query"@nl;
.
elmo:html		a	owl:DatatypeProperty;
	rdfs:label			"html"@en;
	rdfs:label			"html"@nl;
	rdfs:comment		"formulates an html formatted document piece to be inserted in a specific appearance. The html document should be a string an may contain a language descriptor for multi-language purposes"@en;
	rdfs:comment		"Formuleert een html geformatteerd documentdeel die ingevoegd wordt bij bepaalde verschijningen. Het html document behoort als string aanwezig te zijn, en mag een taal-aanduiding bevatten voor meertalige toepassingen"@nl;
.
elmo:contains		a	owl:ObjectProperty;
	rdfs:label			"contains"@en;
	rdfs:label			"bevat"@nl;
	rdfs:comment		"states that a representation contains another representation. This enables the placement of multiple queries on one webpage"@en;
	rdfs:comment		"stelt dat een representatie een andere representatie bevat. Dit maakt het mogelijk om meerdere queries op 1 webpagina te zetten"@nl;
.
elmo:appearance		a	owl:ObjectProperty;
	rdfs:label			"appearance"@en;
	rdfs:label			"verschijning"@nl;
	rdfs:comment		"states that a representation conforms to a certain appearance"@en;
	rdfs:comment		"stelt dat een representatie er uitziet volgens een bepaalde verschijning"@nl;
.
elmo:index			a	owl:DatatypeProperty;
	rdfs:label			"index"@en;
	rdfs:label			"index"@nl;
	rdfs:comment		"the position of a representation that is contained in another representation. Optional field. Representations without an index are always last, but without any other. The 'parent' representation always has a index of '0'. The representation with the lowest number is used in data respresentations (such as ttl, json, etc)."@en;
	rdfs:comment		"de positie van een representatie die onderdeel is van een andere representatie. Optioneel veld. Representaties zonder een index staan achteraan, maar zonder enige volgorde. De 'ouder' representatie heeft altijd een index van '0'. De representatie met het laagste nummer wordt gebruikt in gegevensrepresentaties (zoals ttl, json, etc)."@nl;
.
elmo:fragment		a	owl:ObjectProperty;
	rdfs:label			"fragment"@en;
	rdfs:label			"fragment"@nl;
	rdfs:comment		"defines a fragment of a representation. This is useful for defining a particular fragment of a representation (like a column in a table)"@en;
	rdfs:comment		"definieert een fragment van een representatie. Dit is bruikbaar voor het definieren van een specifiek fragment van een representatie (zoals een kolom van een tabel)"@nl;
.
elmo:layer			a	owl:DatatypeProperty;
	rdfs:label			"layer"@en;
	rdfs:label			"laag"@nl;
	rdfs:comment		"the layer of a representation. Only representations at the highest available layer are used for a specific resource. The lowest layer is the BottomLayer, representations without a layer are considered to be located at the DefaultLayer"@en;
	rdfs:comment		"de laag van een representatie. Alleen representaties op de bovenste beschikbare laag worden gebruikt voor een specifieke resource. De laagste laag is de BottomLayer, representaties zonder een laag bevinden zich op de DefaultLayer"@nl;
.
elmo:name			a	owl:DatatypeProperty;
	rdfs:label			"name"@en;
	rdfs:label			"naam"@nl;
	rdfs:comment		"defines the name of a (fragment of a) representation. This is useful for naming parameters in a html link"@en;
	rdfs:comment		"definieert de naam van een (fragment van een) representatie. Dit is bruikbaar voor het benoemen van parameters in een html link"@nl;
.
elmo:representation	a	owl:ObjectProperty;
	rdfs:label			"representation"@en;
	rdfs:label			"representatie"@nl;
	rdfs:comment		"defines the representation that is used to display a container"@en;
	rdfs:comment		"definieert de representatie die gebruikt wordt om de container af te beelden"@nl;
.
elmo:updates		a	owl:ObjectProperty;
	rdfs:label			"updates"@en;
	rdfs:label			"wijzigt"@nl;
	rdfs:comment		"defines the graph that is updated with the contents of the container. Any old triples for a particular combination of subject en predicate will be replaces with the new ones in the container. All other triples will remain the same."@en;
	rdfs:comment		"definieert de graaf die wordt vernieuwd met de inhoud van de container. Alle oude triples voor een combinatie van subject en predicate worden vervangen door de nieuwe triples uit de container. Alle andere triples blijven hetzelfde."@nl;
.
elmo:partOf			a	owl:ObjectProperty;
	rdfs:label			"part of"@en;
	rdfs:label			"onderdeel van"@nl;
	rdfs:comment		"defines that a container is part of another graph. Only this container-part will be replaced in this graph."@en;
	rdfs:comment		"definieert dat een container onderdeel is van een andere graaf. Alleen dit container-gedeelte wordt vervangen in deze graaf."@nl;
.
elmo:replaces		a	owl:ObjectProperty;
	rdfs:label			"replaces"@en;
	rdfs:label			"vervangt"@nl;
	rdfs:comment		"defines the graph which contents are replaced by the contents of the container"@en;
	rdfs:comment		"definieert de graaf waarvan de inhoud wordt vervangen door de inhoud van de container"@nl;
.
elmo:queryForm		a	owl:ObjectProperty;
	rdfs:label			"query form"@en;
	rdfs:label			"vraagformulier"@nl;
	rdfs:comment		"defines the form that is used when a mandatory URL parameter has no value."@en;
	rdfs:comment		"definieert het formulier dat wordt gebruikt als een verplichte URL parameter geen waarde heeft."@nl;
.
elmo:constraint		a	owl:ObjectProperty;
	rdfs:label			"contraint"@en;
	rdfs:label			"beperking"@nl;
	rdfs:comment		"defines a constraint for a fragment"@en;
	rdfs:comment		"definieert een verplichting voor een fragment"@nl;
.
elmo:use			a	owl:ObjectProperty;
	rdfs:label			"use"@en;
	rdfs:label			"gebruik"@nl;
	rdfs:comment		"defines a custom parameter for a hyperlink. The value of the property will be used, the name will be the name of the property (the part after the '#')"@en;
	rdfs:comment		"definieert een extra parameter voor een hyperlink. De waarde van de eigenschap zal gebruikt worden, de naam van de parameter wordt de naam van de eigenschap (het gedeelte na de '#')"@nl;
.
elmo:file			a	owl:DatatypeProperty;
	rdfs:label			"file"@en;
	rdfs:label			"bestand"@nl;
	rdfs:comment		"defines the file that contains the data used. The file should be placed in the /ldt/data folder"@en;
	rdfs:comment		"defineert een bestand dat de data bevat. Het bestand moet geplaatst worden in de /ldt/data map"@nl;
.
elmo:endpoint		a	owl:ObjectProperty;
	rdfs:label			"endpoint"@en;
	rdfs:label			"endpoint"@nl;
	rdfs:comment		"defines a custom SPARQL endpoint to be used, instead of the regular endpoint (as defined in the defaults.xml configuration file)."@en;
	rdfs:comment		"definieert een alternatief SPARQL endpoint, in plaats van het normale endpoint (zoals gedefinieerd in het defaults.xml configuratiebestand)."@nl;
.
elmo:container		a	owl:ObjectProperty;
	rdfs:label			"container"@en;
	rdfs:label			"container"@nl;
	rdfs:comment		"defines the container that will be used to update the changes made to a representation."@nl;
	rdfs:comment		"definieert de container die gebruikt wordt voor de wijzigingen die gemaakt zijn aan een representatie."@en;
.
elmo:valuesFrom		a	owl:ObjectProperty;
	rdfs:label			"values from"@en;
	rdfs:label			"waarden uit"@nl;
	rdfs:comment		"defines that a picklist in a form should only contain values from another representation"@en;
	rdfs:comment		"defineert dat een invoerveld op een formulier alleen waarden mag bevatten uit een andere representatie"@nl;
.
elmo:valueDatatype	a	owl:ObjectProperty;
	rdfs:label			"values datatype"@en;
	rdfs:label			"datatype van de waarde"@nl;
	rdfs:comment		"defines the datatype of the value that a user can enter in a field on a form. Usable datatypes are dctypes:Dataset, xs:String and xs:Date."@en;
	rdfs:comment		"defineert het datatype van de waarde die een gebruiker kan invoeren in een invoerveld op een formulier. Bruikbare datatypes zijn: dctypes:Dataset, xs:String en xs:Date."@en;
.
elmo:style			a	owl:ObjectProperty;
	rdfs:label			"style"@en;
	rdfs:label			"stijl"@nl;
	rdfs:comment		"defines the style of a fragment"@en;
	rdfs:comment		"defineert de stijl van een fragment"@nl;
.
elmo:template		a	owl:DatatypeProperty;
	rdfs:label			"template"@en;
	rdfs:label			"sjabloon"@nl;
.
elmo:translator		a	owl:ObjectProperty;
	rdfs:label			"translator"@en;
	rdfs:label			"vertaler"@nl;
	rdfs:comment		"defines the translator to be used to translate an uploaded file to linked data"@en;
	rdfs:comment		"definieert de vertaler die gebruikt wordt bij het vertalen van een geuploaded bestand naar linked data"@nl;
.

}

GRAPH elmo:Config {
####################################################################################################

  # Vocabulary for ELMO version 2.0: Extendable Lightweight Model Ontology. A vocabulary for the dotwebstack framework configuration
  #
  # The vocabulary consists of three separate parts:
  # - The system configuration of the framework
  # - The configuration for the backend and core layers of the framework
  # - The configuration for the frontend of the framework
  #
  #
  # This vocabulary file contains the ontology description
  # A complementary file contains the shape graph that should be used when creating statements using this vocabulary.
  #

  # =========
  # Imports
  #
  xsd:string a rdfs:Datatype.
  xsd:integer a rdfs:Datatype.

  # =========
  # Ontology spec
  #
  elmo: a owl:Ontology;
  	rdfs:label "The Extendable Lightweight Model Ontology (ELMO)"@en;
  	rdfs:comment "A vocabulary for the dotwebstack framework configuration."@en;
  	sh:declare [
  		sh:prefix "elmo";
  		sh:namespace "http://dotwebstack.org/def/elmo#"
  	];
  	sh:suggestedShapesGraph <http://dotwebstack.org/def/elmo-shacl#>
  .

  # =========
  # System configuration vocabulary
  #
  elmo:Theatre a owl:Class;
  	rdfs:label "Theatre"@en;
  	rdfs:comment "The class of executable instances for the dotwebstack framework. The system configuration graph should contain exactly one theatre instance. If no theatre instance is present, a default version is created. All sites in the same system configuration graph are considered part of the particular theatre instance."@en;
  .
  elmo:Site a owl:Class;
  	rdfs:label "Site"@en;
  	rdfs:comment "The class of sites that host the dotwebstack framework. A site is identified by a domain name. If no site is present in the system configuration graph, a default version is created, identified by 'localhost'";
  .
  elmo:Stage a owl:Class;
  	rdfs:label "Stage"@en;
  	rdfs:comment "The class of stages at a site. A stage is identified by its site and a base path, the first part of the path after the domain name, typically up to the next slash. If no stage is present, a default version is created, the 'main stage', identified by an empty path.";
  .
  elmo:Layout a owl:Class;
  	rdfs:label "Layout"@en;
  	rdfs:comment "The layout that is used for a particular stage, site or theatre. The theatre layout is inherited by all sites (unless stated otherwise), and a site layout is inherited by all stages for that site (unless stated otherwise). A default layout is used if no layout is specified"@en;
  .

  elmo:domain a owl:DatatypeProperty;
  	rdfs:label "domain"@en;
  	rdfs:comment "States the domain for a particular site"@en;
  	rdfs:domain elmo:Site;
  	rdfs:range xsd:string;
  .
  elmo:site a owl:ObjectProperty;
  	rdfs:label "site"@en;
  	rdfs:comment "States the site to which a particular stage belongs"@en;
  	rdfs:domain elmo:Stage;
  	rdfs:range elmo:Site;
  .
  elmo:basePath a owl:DatatypeProperty;
  	rdfs:label "base path"@en;
  	rdfs:comment "States the base path of a stage, the first part of the path after the domain name, typically up to the next slash. A base path may include slashes";
  .
  elmo:layout a owl:DatatypeProperty;
  	rdfs:label "layout"@en;
  	rdfs:comment "States the layout for a particular theatre, site or stage"@en;
  	rdfs:range elmo:Layout
  	# No rdfs:domain -> domain could be theatre, site or stage
  .

  # =========
  # Backstage and core layers vocabulary
  #
  elmo:InformationProduct a owl:Class;
  	rdfs:label "Information product"@en;
  	rdfs:comment "The class of information product specifications. An information product retrieves some data according to a specific information request, and returns a set of one or more graphs OR a binding set. It should not be possible to use an information product to manipulate data."@en;
  .
  elmo:Transaction a owl:Class;
  	rdfs:label "Transaction"@en;
  	rdfs:comment "The class of transaction specifications. A transaction creates or deletes data according to a specific transaction request. A transaction is defined as a sequence of tasks."@en;
  .
  elmo:Query a owl:Class;
  	rdfs:label "Query"@en;
  	rdfs:comment "Reification of the query. This makes it possible to reuse a query, or to add metadata to the query";
  .

  elmo:Parameter a owl:Class;
  	rdfs:label "Parameter"@en;
  	rdfs:comment "The class of parameters. A parameter is used as input for an information product. Its value(s) are merged with the query according to a template specification.";
  .
  elmo:TermFilter a owl:Class;
  	rdfs:subClassOf elmo:Parameter;
  	rdfs:label "Term filter"@en;
  	rdfs:comment "The class of term filters. A term filter is a parameter that can hold one value and can be used to filter the results of an information product. The value might be a URI or a literal with any datatype."
  .

  elmo:StorageProtocol a owl:Class;
  	rdfs:label "StorageProtocol"@en;
  	rdfs:comment "The class of storage protocols. Instances of this class define how a transactionresult is stored within the persistancy layer";
  .
  elmo:Transformer a owl:Class;
  	rdfs:label "Transformer"@en;
  	rdfs:comment "The class of transformers.";
  .
  elmo:RMLTransformer a owl:Class;
  	rdfs:label "RMLTransformer"@en;
  	rdfs:subClassOf elmo:Transformer;
  	rdfs:comment "The class of RML transformers.";
  .
  elmo:XSLTransformer a owl:Class;
  	rdfs:label "XSLTransformer"@en;
  	rdfs:subClassOf elmo:Transformer;
  	rdfs:comment "The class of XSL transformers.";
  .

  elmo:Backend a owl:Class;
  	rdfs:label "Backend"@en;
  	rdfs:comment "The class of backend specifications. A backend specification specifies the data store that can be accessed to retrieve data or to manipulate the data in the store"@en;
  .
  elmo:SparqlBackend a owl:Class;
  	rdfs:subClassOf elmo:Backend;
  	rdfs:label "Sparql backend"@en;
  	rdfs:comment "The class of sparql backends. A sparql backend implements the sparql 1.1 protocol: http://www.w3.org/TR/sparql11-protocol"@en;
  .
  elmo:ElasticSearchBackend a owl:Class;
  	rdfs:subClassOf elmo:Backend;
  	rdfs:label "Elastic search backend"@en;
  	rdfs:comment "The class of elastic search backends. An Elastic search backend retrieves Linked Data documents from an elastic search server."@en;
  .
  elmo:FileBackend a owl:Class;
  	rdfs:subClassOf elmo:Backend;
  	rdfs:label "File backend"@en;
  	rdfs:comment "The class of file backends. A file backend retrieves Linked Data documents from a file system."@en;
  .

  elmo:backend a owl:ObjectProperty;
  	rdfs:label "backend"@en;
  	rdfs:comment "States the backend for a particular information product"@en;
  	rdfs:range elmo:Backend;
  	# No rdfs:domain -> domain could be information product or transaction, and we may introduce 'source' as a class between information product and backend
  .
  elmo:endpoint a owl:DatatypeProperty;
  	rdfs:label "endpoint"@en;
  	rdfs:comment "States the (http) endpoint that should be accessed for this particular backend. Note: this property is only relevant for backends that respond to http requests"@en;
  	rdfs:domain elmo:Backend;
  	rdfs:range xsd:anyURI;
  .
  elmo:query a owl:DatatypeProperty;
  	rdfs:label "query"@en;
  	rdfs:comment "States the query that specifies the information request. Note: the syntax for a query may differ between backends (for example: a SPARQL query for a Sparql backend, a JSON query for an Elastic search backend)."@en;
  	rdfs:domain elmo:InformationProduct;
  	rdfs:range xsd:string;
  .

  elmo:targetGraph a owl:ObjectProperty;
  	rdfs:label "targetGraph"@en;
  	rdfs:comment "States the named graph that is affected by the transaction. If no target graph is mentioned, and the storageProtocol needs one, the value of the subject parameter is used";
  	rdfs:domain elmo:Transaction;
  	rdfs:range rdfs:Resource;
  .
  elmo:storageProtocol a owl:ObjectProperty;
  	rdfs:label "storageProtocol"@en;
  	rdfs:comment "Defines the way that the result of a transaction is stored within the persistancy layer";
  	rdfs:domain elmo:Transaction;
  	rdfs:range elmo:StorageProtocol;
  .
  elmo:transformer a owl:ObjectProperty;
  	rdfs:label "transformer"@en;
  	rdfs:comment "States the transformer that is used to transform the input data into RDF to store in the in memory transaction dataset";
  	rdfs:domain elmo:Transaction;
  	rdfs:range elmo:Transformer;
  .
  elmo:uriTemplate a owl:DatatypeProperty;
  	rdfs:label "uriTemplate"@en;
  	rdfs:comment "Specifies the template that is used for minting a URI during a transaction.";
  .
  elmo:optionalParameter a owl:ObjectProperty;
  	rdfs:label "optional parameter";
  	rdfs:comment "States the optional parameter(s) for an information product, transaction or query";
  	rdfs:range elmo:Parameter;
  .
  elmo:requiredParameter a owl:ObjectProperty;
  	rdfs:label "required parameter";
  	rdfs:comment "States the optional parameter(s) for an information product, transaction or query";
  	rdfs:range elmo:Parameter;
  .

  # =========
  # Storage protocols
  #
  # Used terminology in the description of the storage protocols:
  # - subject parameter: the parameter that identifies the subject of the transaction. In REST API's this will be similar to the URL
  # - target graph: the URI of an explicitly specified target graph (as part of the transaction configuration), or the value of the subject parameter in case no target graph is specified
  # - transaction dataset: the in memory dataset that is loaded from the http request body (and may be changed by an pre-query)
  #
  elmo-sp:DeleteGraph a elmo:StorageProtocol;
  	rdfs:label "Clear graph";
  	rdfs:comment "Clears the content of the target graph";
  .
  elmo-sp:ReplaceGraph a elmo:StorageProtocol;
  	rdfs:label "Replace graph";
  	rdfs:comment "Replaces the content of the target graph with the content of the transaction dataset";
  .
  elmo-sp:InsertIntoGraph a elmo:StorageProtocol;
  	rdfs:label "Insert into graph";
  	rdfs:comment "Inserts the content of the transaction dataset in the target graph, without deleting any triples in the target graph";
  .
  elmo-sp:InsertOrReplaceResourceInGraph a elmo:StorageProtocol;
  	rdfs:label "Insert or replace resource in graph";
  	rdfs:comment "Insert the content of the transaction dataset in the target graph, and deletes any triples <s,p,o> for any s that is present in the transaction dataset";
  .
  elmo-sp:DeleteResourceFromGraph a elmo:StorageProtocol;
  	rdfs:label "Delete resource from graph";
  	rdfs:comment "Deletes any triples <s,p,o> from the target graph where s is equal to the value of the subject parameter";
  .
  elmo-sp:CreateResourceInGraph a elmo:StorageProtocol;
  	rdfs:label "Create resource in graph";
  	rdfs:comment "mints URIs for any resource in the transaction dataset (as defined by elmo:uriTemplate), and inserts the transaction dataset into the target graph.";
  .
  elmo-sp:InsertIntoVersionGraph a elmo:StorageProtocol;
  	rdfs:label "Insert into version graph";
  	rdfs:comment "inserts the content of the transaction dataset into a newly created versioned target graph.";
  .
  elmo-sp:InvalidateVersionGraph a elmo:StorageProtocol;
  	rdfs:label "Invalidate version graph";
  	rdfs:comment "invalidates the current version (this created a new version that states that the previous version is invalid)";
  .
  elmo-sp:DeleteVersionGraph a elmo:StorageProtocol;
  	rdfs:label "Delete version graph";
  	rdfs:comment "deletes a particular version graph.";
  .
  elmo-sp:CreateResourceInVersionGraph a elmo:StorageProtocol;
  	rdfs:label "Create resource in version graph";
  	rdfs:comment "mints URIs for any resource in the transaction dataset (as defined by elmo:uriTemplate), and inserts the content of the transaction dataset into a newly created versioned target graph.";
  .

  # =========
  # Frontend vocabulary
  #
  elmo:Redirection a owl:Class;
  	rdfs:label "Redirection"@en;
  	rdfs:comment "The class of redirections. A redirection redirects a http request to another URL via the http 303 response"@en;
  .

  elmo:Representation a owl:Class;
  	rdfs:label "Representation"@en;
  	rdfs:comment "The class of representations. A representation links a http request to the corresponding information product."@en;
  .
  elmo:name a owl:DatatypeProperty;
  	rdfs:label "name"@en;
  	rdfs:comment "The unique name of a resource, within a certain context";
  	# No rdfs:domain, name can be used in a lot of situations;
  	rdfs:range xsd:string;
  .
  elmo:urlPattern a owl:DatatypeProperty;
  	rdfs:label "URL pattern"@en;
  	rdfs:comment "Specifies the URL pattern for which this representation should be used. The URL pattern is matched to the part of the http request after removing the domain name of the site and the base path of the stage."@en;
  	# No rdfs:domain, a urlPattern can be used with elmo:Representation and elmo:Redirection
  	rdfs:range xsd:string;
  .
  elmo:uriPattern a owl:DatatypeProperty;
  	rdfs:label "URI pattern"@en;
  	rdfs:comment "Specifies the URI pattern of the subject resource for which this representation should be used. The subject is equal to a dereferenceable URI or the value of the 'subject' or URL parameter if present. In all other cases, no match will be made."@en;
  	rdfs:domain elmo:Representation;
  	rdfs:range xsd:string;
  .
  elmo:appliesTo a owl:ObjectProperty;
  	rdfs:label "applies to"@en;
  	rdfs:comment "Specifies the resource profile for which this representation should be used. A resource profile is a set of triples ([]?p?o). A particular resource ?s matches a resource profile if and only if all triples ?s?p?o exist. For example: the resource profile [rdf:type skos:Concept] whould match any resource that is of type skos:Concept."@en;
  	# no rdfs:domain: it could be elmo:Representation, but also elmo:Fragment;
  	rdfs:range rdfs:Resource;
  .
  elmo:targetUrl a owl:DatatypeProperty;
  	rdfs:label "target URL"@en;
  	rdfs:comment "Specifies the template for the URL to redirect to. The template conforms to the 'replacement' parameter of the string.replaceAll(regex,replacement) method, the elmo:urlPattern will be used as the 'regex' parameter."
  .
  elmo:fragment a owl:ObjectProperty;
  	rdfs:label "fragment"@en;
  	rdfs:comment "Links a particular fragment definition to a representation";
  	rdfs:domain elmo:Representation;
  	rdfs:range elmo:Fragment;
  .
  elmo:informationProduct a owl:ObjectProperty;
  	rdfs:label "information product"@en;
  	rdfs:comment "States the information product of a particular representation"@en;
  	rdfs:domain elmo:Representation;
  	rdfs:range elmo:InformationProduct;
  .
  elmo:putTransaction a owl:ObjectProperty;
  	rdfs:label "transaction"@en;
  	rdfs:comment "States the transaction that is executed for a particular representation, in case of a PUT http request"@en;
  	rdfs:domain elmo:Representation;
  	rdfs:range elmo:Transaction;
  .
  elmo:postTransaction a owl:ObjectProperty;
  	rdfs:label "transaction"@en;
  	rdfs:comment "States the transaction that is executed for a particular representation, in case of a POST http request"@en;
  	rdfs:domain elmo:Representation;
  	rdfs:range elmo:Transaction;
  .
  elmo:deleteTransaction a owl:ObjectProperty;
  	rdfs:label "transaction"@en;
  	rdfs:comment "States the transaction that is executed for a particular representation, in case of a DELETE http request"@en;
  	rdfs:domain elmo:Representation;
  	rdfs:range elmo:Transaction;
  .
  elmo:data a owl:ObjectProperty;
  	rdfs:label "data"@en;
  	rdfs:comment "Links the representation with some particular resource that is used as static data"@en;
  	rdfs:domain elmo:Representation;
  	rdfs:range rdfs:Resource;
  .
  elmo:contains a owl:ObjectProperty;
  	rdfs:label "contains"@en;
  	rdfs:comment "States that a certain top level representation contains child representations. These child representations are only used to give extra information for humans. For non-html serializations, only the information product that is directly linked to the top level representation is used as the data source. The contains-relationship might be used for link headers."@en;
  	rdfs:domain elmo:Representation;
  	rdfs:range elmo:Representation;
  .
  elmo:template a owl:DatatypeProperty;
  	rdfs:label "template"@en;
  	rdfs:comment "Specifies an optional JSX template for the representation. This template replaces a default generated template from the configuration";
  	rdfs:domain elmo:Representation;
  	rdfs:range xsd:string;
  .

  elmo:Fragment a owl:Class;
  	rdfs:label "Fragment"@en;
  	rdfs:comment "The class of fragments";
  .

  elmo:Appearance a owl:Class;
  	rdfs:label "Appearance"@en;
  	rdfs:comment "The class of appearances";
  .
}
